\documentclass{standalone}
\begin{document}
\subsection{Aufgabe 8.4}
\begin{itemize}
	\item[a)]
	$\frac{A}{x^2}$+$\frac{B}{(x^2+1)}+\frac{C}{(x^2+1)^2}$\\
	$A=1, B=0, C=-2$
	\item[b)]
	$\frac{A}{(1+x)}+\frac{Bx+C}{(1+x^2)}$\\
	$A,B,C=\frac{1}{2}$
	\item[c)]
	$\frac{A}{x}+\frac{(Bx+C)}{(x^2+1)}$\\
	$A=-4, B=4, C=1$
	\item[d)]
	$\frac{A}{(x+1)}+\frac{B}{(1-x)}+\frac{C}{1+x}$\\
	$A+C=-1$(kann man A und C im Nenner derselbe Bruh(!) setzsen)$B=1$
	\item[e)]
	$\frac{A}{(x+1)}+\frac{Bx+C}{2x^2-2x+5}$\\
	$A=-1 B=2 C=5$
	\item[f)]
	$\frac{A}{(x+1)}+\frac{B}{(x+1)^2}+\frac{C}{(x^2+1)}+\frac{D}{(x^2+1)^2}$\\
	$A=0, B=-2, C=2, D=-2$
	\item[g)]
	???
	\item[h)]
	$\frac{A}{x}+\frac{B}{x-1}+\frac{C}{(x-1)^2}+\frac{D}{(x-1)^3}$\\
	$A=-1, B=2, C=1, D=2$
	\item[i)]
	$$\frac{A}{x+1}+\frac{Bx+C}{(x^2-x+1)}$$\\
	$A=\frac{2}{3}, B=\frac{1}{3}, C=\frac{1}{3}$
	
\end{itemize}
\end{document}