\documentclass{standalone}
\begin{document}

\subsection{Aufgabe 6.2}
$A + C =  
	\left(\begin{array}{rrr} 
		-1 & 7 \\
		4 & -1 \\
		2 & 10 \\
	\end{array}\right)$
	, $ 2B = \left(\begin{array}{rr}
		6 & 0 \\
		2 & -14\\
	\end{array}\right)$, 
	$B^3=$ $\left(\begin{array}{rr}
		27 & 0 \\
		37 & -343 \\
	\end{array}\right)$,

 
	$A(y+z)= A \left(\left(\begin{array}{r}
		8\\
		-5\\
		\end{array}\right) +
	\left(\begin{array}{r}
		3\\
		2\\
		\end{array}\right)\right)$ =
	$\left(\begin{array}{r}
		-31\\
		41\\
		-26\\
		\end{array}\right)$,
	
	
	$C(-4y)=
	\left(\begin{array}{r}
		-44\\
		 16\\
		-76\\
	\end{array}\right)$,


	$(A+C)\cdot y =	
	\left(\begin{array}{rr}
		-1 & 7 \\
		4 & -1 \\
		2 & 10 \\
	\end{array}\right)$	
		$\cdot
	 \left(\begin{array}{r}
	 	8\\
	 	-5\\
	 \end{array}\right)$ = 
  $ \left(\begin{array}{r}
  	-43\\
  	37\\
  	-34\\
  \end{array}\right)$


	$A \cdot B = 
	\left(\begin{array}{rr}
		-3 & -21 \\
		13 & -7 \\
		2 & -35 \\
	\end{array}\right)$

	$B\cdot C = undefiniert $ 
	
	
	Produkt undefiniert, da 2x2-Matrix mit 3x2-Matrix multipliziert nicht definiert. 
\end{document}
